% -*- LaTeX -*- $Id$

\documentclass{article}[10pt]
\input{macros}
\begin{document}

\title{Spin matrix elements in the $Z_2$ basis}

\author{I. P. McCulloch}
\date{2010}

\maketitle

We define the $Z_2$ symmetric basis as symmetric and antisymmetric
combinations, starting from some states of total spin $j$
with projection onto the $z$ axis of $m$,
\begin{equation}
\begin{array}{rcl}
\ket{m,s} &=& \frac{1}{\sqrt{2}}\left( \ket{m} \: + \: \ket{-m} \right) \\
\ket{m,a} &=& \frac{1}{\sqrt{2}}\left( \ket{m} \: - \: \ket{-m} \right)
\end{array}
\end{equation}
for $m+j$ integer, $m \geq 1/2$, and if $j$ is integer then
also the state $\ket{0,s} = \ket{0}$.
$\ket{0,a}$ doesn't exist.
%
Starting from the matrix elements $S^+\ket{m} = \sqrt{(j-m)(j+m+1)}\ket{m+1}$
and $S^-\ket{m} = \sqrt{(j+m)(j-m+1)}\ket{m-1}$, we construct
the matrix elements of $S^x$ and $S^y$.

Now, $S^x = \frac{S^+ + S^-}{2}$, and we have
\[
(S^+ + S^-)\ket{m,s} = \sqrt{(j-m)(j+m+1)} \ket{m+1,s}
+ \sqrt{(j+m)(j-m+1)} \ket{m-1,s}
\]
%
Also, we have
\[
(S^+ + S^-)\ket{m,a} = \sqrt{(j-m)(j+m+1)} \ket{m+1,a}
+ \sqrt{(j+m)(j-m+1)} \ket{m-1,a}
\]
We must be careful here: if $m \leq 1$, then we need
to keep in mind that $\ket{m-1,a} = -\ket{-m+1,a}$.
%
Notice that the matrix elements that are off-diagonal with 
respect to $a$, $s$ vanish, which implies that
$S^x$ transforms as a scalar (invariant) with respect to
$Z_2$ spin reflection about the $z$-axis.

We can now write down the matrix elements of $S^x$,
\begin{equation}
\begin{array}{rcl}
\bigbraket{m+1,s}{S^x}{m,s} &=& \sqrt{(j-m)(j+m+1)}/2 \\
\bigbraket{m-1,s}{S^x}{m,s} &=& \sqrt{(j+m)(j-m+1)}/2 \\
\bigbraket{m+1,a}{S^x}{m,a} &=& \sqrt{(j-m)(j+m+1)}/2 \\
\bigbraket{m-1,a}{S^x}{m,a} &=& \sqrt{(j+m)(j-m+1)}/2 \\
\end{array}
\end{equation}

Matrix elements involving spins $m=0,1/2,1$ need special treatment.
\begin{equation}
(S+^+S^-)\ket{0,s} = \sqrt{2j(j+1)} \ket{1,s}
\end{equation}
Hence
\begin{equation}
\begin{array}{rcl}
\bigbraket{1,s}{S^x}{0,s} &=& \sqrt{j(j+1)/2} \\
\bigbraket{0,s}{S^x}{1,s} &=& \sqrt{j(j+1)/2} \\
\end{array}
\end{equation}
And note that the factor 2 is inside the square root.
%
Matrix elements for $m=1/2$ are diagonal and simplify,
\begin{equation}
\begin{array}{rcl}
\bigbraket{1/2,s}{S^x}{1/2,s} &=&phantom{-}(j+1/2)/2 \\
\bigbraket{1/2,a}{S^x}{1/2,a} &=& -(j+1/2)/2
\end{array}
\end{equation}
which gives the novelty of a matrix element which is negative
(although that follows from $S^x$ being diagonal in this representation,
since the spin matrices are always traceless).

Now we repeat the analysis for $2iS^y = S^+ - S^-$.
\[
(S^- + S^-)\ket{m,s} = \sqrt{(j-m)(j+m+1)} \ket{m+1,a}
- \sqrt{(j+m)(j-m+1)} \ket{m-1,a}
\]
\[
(S^+ - S^-)\ket{m,a} = \sqrt{(j-m)(j+m+1)} \ket{m+1,s}
- \sqrt{(j+m)(j-m+1)} \ket{m-1,s}
\]
which gives
\begin{equation}
\begin{array}{rcl}
\bigbraket{m+1,a}{S^y}{m,s} &=& -i\sqrt{(j-m)(j+m+1)}/2 \\
\bigbraket{m-1,a}{S^y}{m,s} &=& \phantom{-}i\sqrt{(j+m)(j-m+1)}/2 \\
\bigbraket{m+1,s}{S^y}{m,a} &=& -i\sqrt{(j-m)(j+m+1)}/2 \\
\bigbraket{m-1,s}{S^y}{m,a} &=& \phantom{-}i\sqrt{(j+m)(j-m+1)}/2 \\
\end{array}
\end{equation}
And, for $m=0$,
\begin{equation}
\begin{array}{rcl}
\bigbraket{1,a}{S^y}{0,s} &=& -i(\sqrt{j(j+1)/2}) \\
\bigbraket{0,s}{S^y}{1,a} &=& \phantom{-}i(\sqrt{j(j+1)/2}) \\
\end{array}
\end{equation}
%
For $m=1/2$, we have
\begin{equation}
\begin{array}{rcl}
\bigbraket{1/2,a}{S^y}{1/2,s} &=& -i(j+1/2)/2 \\
\bigbraket{1/2,s}{S^y}{1/2,a} &=& \phantom{-}i(j+1/2)/2 \\
\end{array}
\end{equation}
We also note that $S^y$ transforms as $a$ under $Z_2$ spin
flip in the $z$-axis.

For completeness, we also write down the matrix elements of $S^z$, which
also transforms as $a$,
\begin{equation}
\begin{array}{rcl}
\bigbraket{m,a}{S^z}{m,s} &=& m \\
\bigbraket{m,s}{S^z}{m,a} &=& m \\
\end{array}
\end{equation}


\end{document}
